Foundation/Modal/Boxdot/GLPoint3_GrzPoint3.lean
@@ -20,7 +20,7 @@ open Formula (boxdotTranslate)
 open Modal.Kripke
 open Entailment
 
-lemma provable_boxdotTranslated_GLPoint3_of_GrzPoint3 : Modal.GrzPoint3 ⊢! φ → Modal.GLPoint3 ⊢! φᵇ := Hilbert.Normal.of_provable_boxdotTranslated_axiomInstances $ by
+lemma provable_boxdotTranslated_GLPoint3_of_GrzPoint3 : Modal.GrzPoint3 ⊢ φ → Modal.GLPoint3 ⊢ φᵇ := Hilbert.Normal.of_provable_boxdotTranslated_axiomInstances $ by
   intro φ hp;
   rcases (by simpa [Axiom.instances] using hp) with (⟨_, _, rfl⟩ | ⟨_, rfl⟩ | ⟨s, _, rfl⟩);
   . exact boxdot_axiomK!;
@@ -74,7 +74,7 @@ lemma provable_boxdotTranslated_GLPoint3_of_GrzPoint3 : Modal.GrzPoint3 ⊢! φ 
       . exact hC₂₂ $ hC₁₁₂ z Ryz;
       . exact hC₁₂ $ hC₂₁₂ y Rzy;
 
-lemma provable_GrzPoint3_of_boxdotTranslated_GLPoint3 : Modal.GLPoint3 ⊢! φᵇ → Modal.GrzPoint3 ⊢! φ := by
+lemma provable_GrzPoint3_of_boxdotTranslated_GLPoint3 : Modal.GLPoint3 ⊢ φᵇ → Modal.GrzPoint3 ⊢ φ := by
   intro h;
   replace h := Sound.sound (𝓜 := FrameClass.finite_GLPoint3) h;
   apply Complete.complete (𝓜 := FrameClass.finite_GrzPoint3);
@@ -89,7 +89,7 @@ lemma provable_GrzPoint3_of_boxdotTranslated_GLPoint3 : Modal.GLPoint3 ⊢! φ�
     apply iff_reflexivize_irreflexivize'.not.mp;
     exact h;
 
-theorem iff_boxdotTranslatedGLPoint3_GrzPoint3 : Modal.GLPoint3 ⊢! φᵇ ↔ Modal.GrzPoint3 ⊢! φ := ⟨
+theorem iff_boxdotTranslatedGLPoint3_GrzPoint3 : Modal.GLPoint3 ⊢ φᵇ ↔ Modal.GrzPoint3 ⊢ φ := ⟨
   provable_GrzPoint3_of_boxdotTranslated_GLPoint3,
   provable_boxdotTranslated_GLPoint3_of_GrzPoint3
 ⟩
