Foundation/Modal/Kripke/AxiomMcK.lean
@@ -23,7 +23,7 @@ open Formula.Kripke
 
 variable {φ ψ : Formula _}
 
-lemma axiomMcK_DiaCDiaBox! : Modal.K ⊢! (□◇φ ➝ ◇□φ) ⭤ ◇(◇φ ➝ □φ) := by
+lemma axiomMcK_DiaCDiaBox! : Modal.K ⊢ (□◇φ ➝ ◇□φ) ⭤ ◇(◇φ ➝ □φ) := by
   apply Complete.complete (𝓜 := Kripke.FrameClass.K);
   intro F _ V x;
   apply Satisfies.iff_def.mpr;
@@ -52,7 +52,7 @@ lemma axiomMcK_DiaCDiaBox! : Modal.K ⊢! (□◇φ ➝ ◇□φ) ⭤ ◇(◇φ 
     . assumption;
     . exact hy $ hx₂ _ Rxy;
 
-lemma CKDiaBoxDiaK! : Modal.K ⊢! (◇φ ⋏ □ψ) ➝ ◇(φ ⋏ ψ) := by
+lemma CKDiaBoxDiaK! : Modal.K ⊢ (◇φ ⋏ □ψ) ➝ ◇(φ ⋏ ψ) := by
   apply Complete.complete (𝓜 := Kripke.FrameClass.K);
   intro F _ V x hx;
   have ⟨hx₁, hx₂⟩ := Satisfies.and_def.mp hx;
@@ -66,7 +66,7 @@ lemma CKDiaBoxDiaK! : Modal.K ⊢! (◇φ ⋏ □ψ) ➝ ◇(φ ⋏ ψ) := by
     . assumption
     . apply hx₂ _ Rxy;
 
-lemma CKBoxDiaDiaK! : Modal.K ⊢! (□φ ⋏ ◇ψ) ➝ ◇(φ ⋏ ψ) := by
+lemma CKBoxDiaDiaK! : Modal.K ⊢ (□φ ⋏ ◇ψ) ➝ ◇(φ ⋏ ψ) := by
   apply Complete.complete (𝓜 := Kripke.FrameClass.K);
   intro F _ V x hx;
   have ⟨hx₁, hx₂⟩ := Satisfies.and_def.mp hx;
@@ -89,33 +89,33 @@ open LO.Entailment Entailment.FiniteContext LO.Modal.Entailment
 
 variable {φ ψ : Formula _}
 
-lemma CKDiaBoxDiaK! : Modal.K4McK ⊢! (◇φ ⋏ □ψ) ➝ ◇(φ ⋏ ψ) := WeakerThan.pbl Logic.K.CKDiaBoxDiaK!
+lemma CKDiaBoxDiaK! : Modal.K4McK ⊢ (◇φ ⋏ □ψ) ➝ ◇(φ ⋏ ψ) := WeakerThan.pbl Logic.K.CKDiaBoxDiaK!
 
-lemma CKBoxDiaDiaK! : Modal.K4McK ⊢! (□φ ⋏ ◇ψ) ➝ ◇(φ ⋏ ψ) := WeakerThan.pbl Logic.K.CKBoxDiaDiaK!
+lemma CKBoxDiaDiaK! : Modal.K4McK ⊢ (□φ ⋏ ◇ψ) ➝ ◇(φ ⋏ ψ) := WeakerThan.pbl Logic.K.CKBoxDiaDiaK!
 
-lemma DiaK!_of_CKBoxDia (h : Modal.K4McK ⊢! ◇φ ⋏ □ψ) : Modal.K4McK ⊢! ◇(φ ⋏ ψ) := CKDiaBoxDiaK! ⨀ h
-lemma DiaK!_of_CKDiaBox (h : Modal.K4McK ⊢! □φ ⋏ ◇ψ) : Modal.K4McK ⊢! ◇(φ ⋏ ψ) := CKBoxDiaDiaK! ⨀ h
+lemma DiaK!_of_CKBoxDia (h : Modal.K4McK ⊢ ◇φ ⋏ □ψ) : Modal.K4McK ⊢ ◇(φ ⋏ ψ) := CKDiaBoxDiaK! ⨀ h
+lemma DiaK!_of_CKDiaBox (h : Modal.K4McK ⊢ □φ ⋏ ◇ψ) : Modal.K4McK ⊢ ◇(φ ⋏ ψ) := CKBoxDiaDiaK! ⨀ h
 
-lemma DiaCDiaBox! : Modal.K4McK ⊢! ◇(◇φ ➝ □φ) :=
+lemma DiaCDiaBox! : Modal.K4McK ⊢ ◇(◇φ ➝ □φ) :=
   (WeakerThan.pbl $ C_of_E_mp! $ Logic.K.axiomMcK_DiaCDiaBox!) ⨀ (by simp)
 
-lemma DiaConjCDiabox {Γ : List _} (hΓ : Γ ≠ []) : Modal.K4McK ⊢! ◇(Γ.map (λ φ => ◇φ ➝ □φ)).conj := by
+lemma DiaConjCDiabox {Γ : List _} (hΓ : Γ ≠ []) : Modal.K4McK ⊢ ◇(Γ.map (λ φ => ◇φ ➝ □φ)).conj := by
   induction Γ using List.induction_with_singleton with
   | hnil => tauto;
   | hsingle φ =>
     apply diaK''! ?_ $ DiaCDiaBox! (φ := φ);
     apply right_K!_intro <;> simp;
   | hcons φ Γ _ ih =>
-    have : Modal.K4McK ⊢! ◇□(◇φ ➝ □φ) ⋏ □◇(List.map (fun φ ↦ (◇φ ➝ □φ)) Γ).conj := by
+    have : Modal.K4McK ⊢ ◇□(◇φ ➝ □φ) ⋏ □◇(List.map (fun φ ↦ (◇φ ➝ □φ)) Γ).conj := by
       apply K!_intro;
       . exact axiomMcK! ⨀ (nec! DiaCDiaBox!);
       . exact nec! $ ih $ by assumption;
-    have : Modal.K4McK ⊢! ◇(□(◇φ ➝ □φ) ⋏ ◇(List.map (fun φ ↦ ◇φ ➝ □φ) Γ).conj) := DiaK!_of_CKBoxDia this;
-    replace : Modal.K4McK ⊢! ◇◇((◇φ ➝ □φ) ⋏ (List.map (fun φ ↦ ◇φ ➝ □φ) Γ).conj) := diaK''! CKBoxDiaDiaK! this;
-    replace : Modal.K4McK ⊢! ◇((◇φ ➝ □φ) ⋏ (List.map (fun φ ↦ ◇φ ➝ □φ) Γ).conj) := diaFour'! this;
+    have : Modal.K4McK ⊢ ◇(□(◇φ ➝ □φ) ⋏ ◇(List.map (fun φ ↦ ◇φ ➝ □φ) Γ).conj) := DiaK!_of_CKBoxDia this;
+    replace : Modal.K4McK ⊢ ◇◇((◇φ ➝ □φ) ⋏ (List.map (fun φ ↦ ◇φ ➝ □φ) Γ).conj) := diaK''! CKBoxDiaDiaK! this;
+    replace : Modal.K4McK ⊢ ◇((◇φ ➝ □φ) ⋏ (List.map (fun φ ↦ ◇φ ➝ □φ) Γ).conj) := diaFour'! this;
     exact this;
 
-lemma DiaFconjCDiabox {Γ : Finset _} (hΓ : Γ ≠ ∅) : Modal.K4McK ⊢! ◇(Γ.image (λ φ => ◇φ ➝ □φ)).conj := by
+lemma DiaFconjCDiabox {Γ : Finset _} (hΓ : Γ ≠ ∅) : Modal.K4McK ⊢ ◇(Γ.image (λ φ => ◇φ ➝ □φ)).conj := by
   apply diaK''! ?_ (h₂ := DiaConjCDiabox (Γ := Γ.toList) ?_);
   . apply right_Fconj!_intro;
     intro ψ hψ;
@@ -195,7 +195,7 @@ instance [Modal.K4McK ⪯ (Hilbert.Normal Ax)] : (canonicalFrame (Hilbert.Normal
     replace hC := FConj_DT.mp hC;
 
     let Γ' := insert (◇⊤ ➝ □⊤) Γ;
-    replace hC : Γ'.toSet *⊢[(Hilbert.Normal Ax)]! ⊥ := Context.weakening! (by simp [Γ']) hC;
+    replace hC : Γ'.toSet *⊢[(Hilbert.Normal Ax)] ⊥ := Context.weakening! (by simp [Γ']) hC;
 
     let Γ'₁ := { φ ∈ Γ' | φ ∈ x.1.1.prebox };
     let Γ'₂ := { φ ∈ Γ' | ∃ ψ, ◇ψ ➝ □ψ = φ };
@@ -208,7 +208,7 @@ instance [Modal.K4McK ⪯ (Hilbert.Normal Ax)] : (canonicalFrame (Hilbert.Normal
       . suffices ∃ φ, ¬φ = ⊤ → ◇φ ➝ □φ ∈ Γ by simpa [Finset.eq_empty_iff_forall_notMem, Γ'];
         use ⊤;
         simp;
-    . replace hC : (Γ'₁ ∪ Γ'₂).toSet *⊢[(Hilbert.Normal Ax)]! ⊥ := by
+    . replace hC : (Γ'₁ ∪ Γ'₂).toSet *⊢[(Hilbert.Normal Ax)] ⊥ := by
         convert hC;
         ext φ;
         simp only [Set.mem_preimage, Function.iterate_one, Finset.mem_union, Finset.mem_filter, Finset.mem_insert, Γ'₁, Γ', Γ'₂];
@@ -219,9 +219,9 @@ instance [Modal.K4McK ⪯ (Hilbert.Normal Ax)] : (canonicalFrame (Hilbert.Normal
           . have := hΓ h;
             simp at this ⊢;
             tauto;
-      replace hC : Γ'₁.toSet.box *⊢[(Hilbert.Normal Ax)]! □(∼Γ'₂.conj) := Context.nec! $ N!_iff_CO!.mpr $ FConj_DT'.mpr hC;
-      replace hC : Γ'₁.box.toSet *⊢[(Hilbert.Normal Ax)]! □(∼Γ'₂.conj) := by convert hC; simp;
-      replace hC : Γ'₁.box.toSet *⊢[(Hilbert.Normal Ax)]! ∼◇(Γ'₂.conj) := by
+      replace hC : Γ'₁.toSet.box *⊢[(Hilbert.Normal Ax)] □(∼Γ'₂.conj) := Context.nec! $ N!_iff_CO!.mpr $ FConj_DT'.mpr hC;
+      replace hC : Γ'₁.box.toSet *⊢[(Hilbert.Normal Ax)] □(∼Γ'₂.conj) := by convert hC; simp;
+      replace hC : Γ'₁.box.toSet *⊢[(Hilbert.Normal Ax)] ∼◇(Γ'₂.conj) := by
         apply FConj_DT.mp;
         apply C!_trans $ FConj_DT.mpr hC;
         simp;
