Foundation/Propositional/Logic/Letterless_Int_Cl.lean
@@ -16,17 +16,17 @@ namespace Logic
 
 open LO.Entailment LO.Entailment.FiniteContext LO.Modal.Entailment
 
-theorem iff_letterless_Int_Cl {φ : Formula ℕ} (hφ : φ.Letterless) : Propositional.Int ⊢! φ ↔ Propositional.Cl ⊢! φ := by
+theorem iff_letterless_Int_Cl {φ : Formula ℕ} (hφ : φ.Letterless) : Propositional.Int ⊢ φ ↔ Propositional.Cl ⊢ φ := by
   constructor;
   . apply WeakerThan.wk;
     infer_instance;
   . intro h;
-    have : Modal.S4 ⊢! ◇φᵍ := Modal.iff_provable_Cl_provable_dia_gS4.mp h;
-    have : Modal.Triv ⊢! ◇φᵍ := WeakerThan.pbl this;
-    have : Modal.Triv ⊢! φᵍ := diaT'! this;
+    have : Modal.S4 ⊢ ◇φᵍ := Modal.iff_provable_Cl_provable_dia_gS4.mp h;
+    have : Modal.Triv ⊢ ◇φᵍ := WeakerThan.pbl this;
+    have : Modal.Triv ⊢ φᵍ := diaT'! this;
     have : (φᵍᵀ.toPropFormula _).isTautology := Modal.Triv.iff_isTautology.mp this;
-    have : Modal.KD ⊢! φᵍ := Modal.Logic.provable_KD_of_classical_tautology (by grind) this;
-    have : Modal.S4 ⊢! φᵍ := WeakerThan.pbl this;
+    have : Modal.KD ⊢ φᵍ := Modal.Logic.provable_KD_of_classical_tautology (by grind) this;
+    have : Modal.S4 ⊢ φᵍ := WeakerThan.pbl this;
     exact Modal.ModalCompanion.companion.mpr this;
 
 end Logic
